MicroPolicies/Instance.v
@@ -1,0 +1,53 @@
+
+From mathcomp Require Import ssreflect ssrfun ssrbool eqtype ssrint seq.
+From CoqUtils Require Import fmap word.
+
+Require Import Int32.
+Require Import LRC.
+Require Import Types.
+Require Import Symbolic.
+Require Import Exec.
+
+Definition mt := concrete_int_32_mt.
+
+Global Instance ops : machine_ops mt := concrete_int_32_ops.
+(* ra := word.as_word 5 *)
+
+Global Instance scr : syscall_regs mt := concrete_int_32_scr.
+(* syscall_ret  := as_word 16;
+   syscall_arg1 := as_word 17;
+   syscall_arg2 := as_word 18;
+   syscall_arg3 := as_word 19 *)
+
+Definition table : @Symbolic.syscall_table mt sym_lrc :=
+  [fmap (as_word 4096, {| Symbolic.entry_tag := tt ; Symbolic.sem := alloc_fun |})].
+(* TL TODO: 4096 is the largest power of 2 that doesn't cause coq stack overflow *)
+(*          could also be syscall addr at the beginning of meemory, but would    *)
+(*          need to chance encoding.                                             *)
+
+Definition state := (@Symbolic.state mt sym_lrc).
+Definition stepf := (@Exec.stepf mt ops sym_lrc table).
+
+Definition ratom := (atom (mword mt) value_tag).
+Definition matom := (atom (mword mt) mem_tag).
+
+(* Machine initialisation *)
+Definition reg0 : {fmap reg mt -> ratom } :=
+  [fmap (as_word 0, Atom (as_word 0) Other)
+      ; (as_word 1, Atom (as_word 0) Other)
+      ; (as_word 2, Atom (as_word 0) Other)
+      ; (as_word 3, Atom (as_word 0) Other)
+      ; (as_word 4, Atom (as_word 0) Other)
+      ; (as_word 5, Atom (as_word 0) Other)
+      ; (as_word 6, Atom (as_word 0) Other)
+      ; (as_word 16, Atom (as_word 0) Other)
+      ; (as_word 17, Atom (as_word 0) Other)
+      ; (as_word 18, Atom (as_word 0) Other)
+      ; (as_word 19, Atom (as_word 0) Other)].
+
+
+Definition load (m : {fmap mword mt -> matom }) : state :=
+  {| Symbolic.mem := m ;
+     Symbolic.regs := reg0 ;
+     Symbolic.pc := {| vala := word.as_word 0 ; taga := Level 0 |} ;
+     Symbolic.internal := tt |}.
